src/compiler_generic/meta_isabelle/Printer_Isabelle.thy
@@ -47,15 +47,15 @@ begin
 context Print
 begin
 
-fun s_of_semi__typ where "s_of_semi__typ e = (\<lambda>
+fun of_semi__typ where "of_semi__typ e = (\<lambda>
     Typ_base s \<Rightarrow> To_string s
-  | Typ_apply name l \<Rightarrow> sprint2 \<open>%s %s\<close>\<acute> (let s = String_concat \<open>, \<close> (List.map s_of_semi__typ l) in
+  | Typ_apply name l \<Rightarrow> sprint2 \<open>%s %s\<close>\<acute> (let s = String_concat \<open>, \<close> (List.map of_semi__typ l) in
                                                  case l of [_] \<Rightarrow> s | _ \<Rightarrow> sprint1 \<open>(%s)\<close>\<acute> s)
-                                                (s_of_semi__typ name)
-  | Typ_apply_bin s ty1 ty2 \<Rightarrow> sprint3 \<open>%s %s %s\<close>\<acute> (s_of_semi__typ ty1) (To_string s) (s_of_semi__typ ty2)
-  | Typ_apply_paren s1 s2 ty \<Rightarrow> sprint3 \<open>%s%s%s\<close>\<acute> (To_string s1) (s_of_semi__typ ty) (To_string s2)) e"
+                                                (of_semi__typ name)
+  | Typ_apply_bin s ty1 ty2 \<Rightarrow> sprint3 \<open>%s %s %s\<close>\<acute> (of_semi__typ ty1) (To_string s) (of_semi__typ ty2)
+  | Typ_apply_paren s1 s2 ty \<Rightarrow> sprint3 \<open>%s%s%s\<close>\<acute> (To_string s1) (of_semi__typ ty) (To_string s2)) e"
 
-definition "s_of_datatype _ = (\<lambda> Datatype n l \<Rightarrow>
+definition "of_datatype _ = (\<lambda> Datatype n l \<Rightarrow>
   sprint2 \<open>datatype %s = %s\<close>\<acute>
     (To_string n)
     (String_concat \<open>
@@ -64,34 +64,34 @@ definition "s_of_datatype _ = (\<lambda> Datatype n l \<Rightarrow>
         (\<lambda>(n,l).
          sprint2 \<open>%s %s\<close>\<acute>
            (To_string n)
-           (String_concat \<open> \<close> (L.map (\<lambda>x. sprint1 \<open>\"%s\"\<close>\<acute> (s_of_semi__typ x)) l))) l) ))"
+           (String_concat \<open> \<close> (L.map (\<lambda>x. sprint1 \<open>\"%s\"\<close>\<acute> (of_semi__typ x)) l))) l) ))"
 
-definition "s_of_type_synonym _ = (\<lambda> Type_synonym n v l \<Rightarrow>
+definition "of_type_synonym _ = (\<lambda> Type_synonym n v l \<Rightarrow>
     sprint2 \<open>type_synonym %s = \"%s\"\<close>\<acute> (if v = [] then 
                                            To_string n
                                          else
-                                           s_of_semi__typ (Typ_apply (Typ_base n) (L.map Typ_base v)))
-                                        (s_of_semi__typ l))"
+                                           of_semi__typ (Typ_apply (Typ_base n) (L.map Typ_base v)))
+                                        (of_semi__typ l))"
 
-fun s_of_semi__term where "s_of_semi__term e = (\<lambda>
-    Term_rewrite e1 symb e2 \<Rightarrow> sprint3 \<open>%s %s %s\<close>\<acute> (s_of_semi__term e1) (To_string symb) (s_of_semi__term e2)
+fun of_semi__term where "of_semi__term e = (\<lambda>
+    Term_rewrite e1 symb e2 \<Rightarrow> sprint3 \<open>%s %s %s\<close>\<acute> (of_semi__term e1) (To_string symb) (of_semi__term e2)
   | Term_basic l \<Rightarrow> sprint1 \<open>%s\<close>\<acute> (String_concat \<open> \<close> (L.map To_string l))
-  | Term_annot e s \<Rightarrow> sprint2 \<open>(%s::%s)\<close>\<acute> (s_of_semi__term e) (s_of_semi__typ s)
-  | Term_bind symb e1 e2 \<Rightarrow> sprint3 \<open>(%s%s. %s)\<close>\<acute> (To_string symb) (s_of_semi__term e1) (s_of_semi__term e2)
+  | Term_annot e s \<Rightarrow> sprint2 \<open>(%s::%s)\<close>\<acute> (of_semi__term e) (of_semi__typ s)
+  | Term_bind symb e1 e2 \<Rightarrow> sprint3 \<open>(%s%s. %s)\<close>\<acute> (To_string symb) (of_semi__term e1) (of_semi__term e2)
   | Term_fun_case e_case l \<Rightarrow> sprint2 \<open>(%s %s)\<close>\<acute>
       (case e_case of None \<Rightarrow> \<open>\<lambda>\<close>
-                    | Some e \<Rightarrow> sprint1 \<open>case %s of\<close>\<acute> (s_of_semi__term e))
+                    | Some e \<Rightarrow> sprint1 \<open>case %s of\<close>\<acute> (of_semi__term e))
       (String_concat \<open>
-    | \<close> (List.map (\<lambda> (s1, s2) \<Rightarrow> sprint2 \<open>%s \<Rightarrow> %s\<close>\<acute> (s_of_semi__term s1) (s_of_semi__term s2)) l))
-  | Term_apply e l \<Rightarrow> sprint2 \<open>%s %s\<close>\<acute> (s_of_semi__term e) (String_concat \<open> \<close> (List.map (\<lambda> e \<Rightarrow> sprint1 \<open>%s\<close>\<acute> (s_of_semi__term e)) l))
-  | Term_paren p_left p_right e \<Rightarrow> sprint3 \<open>%s%s%s\<close>\<acute> (To_string p_left) (s_of_semi__term e) (To_string p_right)
-  | Term_if_then_else e_if e_then e_else \<Rightarrow> sprint3 \<open>if %s then %s else %s\<close>\<acute> (s_of_semi__term e_if) (s_of_semi__term e_then) (s_of_semi__term e_else)
-  | Term_term l pure \<Rightarrow> s_of_pure_term (L.map To_string l) pure) e"
+    | \<close> (List.map (\<lambda> (s1, s2) \<Rightarrow> sprint2 \<open>%s \<Rightarrow> %s\<close>\<acute> (of_semi__term s1) (of_semi__term s2)) l))
+  | Term_apply e l \<Rightarrow> sprint2 \<open>%s %s\<close>\<acute> (of_semi__term e) (String_concat \<open> \<close> (List.map (\<lambda> e \<Rightarrow> sprint1 \<open>%s\<close>\<acute> (of_semi__term e)) l))
+  | Term_paren p_left p_right e \<Rightarrow> sprint3 \<open>%s%s%s\<close>\<acute> (To_string p_left) (of_semi__term e) (To_string p_right)
+  | Term_if_then_else e_if e_then e_else \<Rightarrow> sprint3 \<open>if %s then %s else %s\<close>\<acute> (of_semi__term e_if) (of_semi__term e_then) (of_semi__term e_else)
+  | Term_term l pure \<Rightarrow> of_pure_term (L.map To_string l) pure) e"
 
-definition "s_of_type_notation _ = (\<lambda> Type_notation n e \<Rightarrow>
+definition "of_type_notation _ = (\<lambda> Type_notation n e \<Rightarrow>
     sprint2 \<open>type_notation %s (\"%s\")\<close>\<acute> (To_string n) (To_string e))"
 
-definition "s_of_instantiation _ = (\<lambda> Instantiation n n_def expr \<Rightarrow>
+definition "of_instantiation _ = (\<lambda> Instantiation n n_def expr \<Rightarrow>
     let name = To_string n in
     sprint4 \<open>instantiation %s :: object
 begin
@@ -101,179 +101,179 @@ end\<close>\<acute>
       name
       (To_string n_def)
       name
-      (s_of_semi__term expr))"
+      (of_semi__term expr))"
 
-definition "s_of_defs _ = (\<lambda> Defs_overloaded n e \<Rightarrow>
-    sprint2 \<open>defs(overloaded) %s : \"%s\"\<close>\<acute> (To_string n) (s_of_semi__term e))"
+definition "of_defs _ = (\<lambda> Defs_overloaded n e \<Rightarrow>
+    sprint2 \<open>defs(overloaded) %s : \"%s\"\<close>\<acute> (To_string n) (of_semi__term e))"
 
-definition "s_of_consts _ = (\<lambda> Consts n ty symb \<Rightarrow>
-    sprint4 \<open>consts %s :: \"%s\" (\"%s %s\")\<close>\<acute> (To_string n) (s_of_semi__typ ty) (To_string Consts_value) (To_string symb))"
+definition "of_consts _ = (\<lambda> Consts n ty symb \<Rightarrow>
+    sprint4 \<open>consts %s :: \"%s\" (\"%s %s\")\<close>\<acute> (To_string n) (of_semi__typ ty) (To_string Consts_value) (To_string symb))"
 
-definition "s_of_definition _ = (\<lambda>
-    Definition e \<Rightarrow> sprint1 \<open>definition \"%s\"\<close>\<acute> (s_of_semi__term e)
+definition "of_definition _ = (\<lambda>
+    Definition e \<Rightarrow> sprint1 \<open>definition \"%s\"\<close>\<acute> (of_semi__term e)
   | Definition_where1 name (abbrev, prio) e \<Rightarrow> sprint4 \<open>definition %s (\"(1%s)\" %d)
-  where \"%s\"\<close>\<acute> (To_string name) (s_of_semi__term abbrev) (To_nat prio) (s_of_semi__term e)
+  where \"%s\"\<close>\<acute> (To_string name) (of_semi__term abbrev) (To_nat prio) (of_semi__term e)
   | Definition_where2 name abbrev e \<Rightarrow> sprint3 \<open>definition %s (\"%s\")
-  where \"%s\"\<close>\<acute> (To_string name) (s_of_semi__term abbrev) (s_of_semi__term e))"
+  where \"%s\"\<close>\<acute> (To_string name) (of_semi__term abbrev) (of_semi__term e))"
 
-definition "(s_of_semi__thm_attribute_aux_gen :: String.literal \<times> String.literal \<Rightarrow> _ \<Rightarrow> _ \<Rightarrow> _) m lacc s = 
+definition "(of_semi__thm_attribute_aux_gen :: String.literal \<times> String.literal \<Rightarrow> _ \<Rightarrow> _ \<Rightarrow> _) m lacc s = 
  (let s_base = (\<lambda>s lacc. sprint2 \<open>%s[%s]\<close>\<acute> (To_string s) (String_concat \<open>, \<close> (L.map (\<lambda>(s, x). sprint2 \<open>%s %s\<close>\<acute> s x) lacc))) in
   s_base s (m # lacc))"
 
-definition "s_of_semi__thm_attribute_aux_gen_where l = 
+definition "of_semi__thm_attribute_aux_gen_where l = 
  (\<open>where\<close>, String_concat \<open> and \<close> (L.map (\<lambda>(var, expr). sprint2 \<open>%s = \"%s\"\<close>\<acute>
                                                             (To_string var)
-                                                            (s_of_semi__term expr)) l))"
+                                                            (of_semi__term expr)) l))"
 
-definition "s_of_semi__thm_attribute_aux_gen_of l =
- (\<open>of\<close>, String_concat \<open> \<close> (L.map (\<lambda>expr. sprint1 \<open>\"%s\"\<close>\<acute> (s_of_semi__term expr)) l))"
+definition "of_semi__thm_attribute_aux_gen_of l =
+ (\<open>of\<close>, String_concat \<open> \<close> (L.map (\<lambda>expr. sprint1 \<open>\"%s\"\<close>\<acute> (of_semi__term expr)) l))"
 
 (* NOTE all 'let' declarations can be put at the beginning *)
    (*let f_where = (\<lambda>l. (\<open>where\<close>, String_concat \<open> and \<close>
                                         (L.map (\<lambda>(var, expr). sprint2 \<open>%s = \"%s\"\<close>\<acute>
                                                         (To_string var)
-                                                        (s_of_semi__term expr)) l)))
+                                                        (of_semi__term expr)) l)))
      ; f_of = (\<lambda>l. (\<open>of\<close>, String_concat \<open> \<close>
                                   (L.map (\<lambda>expr. sprint1 \<open>\"%s\"\<close>\<acute>
-                                                        (s_of_semi__term expr)) l)))
+                                                        (of_semi__term expr)) l)))
      ; f_symmetric = (\<open>symmetric\<close>, \<open>\<close>)
      ; s_base = (\<lambda>s lacc. sprint2 \<open>%s[%s]\<close>\<acute> (To_string s) (String_concat \<open>, \<close> (L.map (\<lambda>(s, x). sprint2 \<open>%s %s\<close>\<acute> s x) lacc))) in
    *)
-fun s_of_semi__thm_attribute_aux where "s_of_semi__thm_attribute_aux lacc e =
+fun of_semi__thm_attribute_aux where "of_semi__thm_attribute_aux lacc e =
   (\<lambda> Thm_thm s \<Rightarrow> To_string s
    | Thm_thms s \<Rightarrow> To_string s
 
-   | Thm_THEN (Thm_thm s) e2 \<Rightarrow> s_of_semi__thm_attribute_aux_gen (\<open>THEN\<close>, s_of_semi__thm_attribute_aux [] e2) lacc s
-   | Thm_THEN (Thm_thms s) e2 \<Rightarrow> s_of_semi__thm_attribute_aux_gen (\<open>THEN\<close>, s_of_semi__thm_attribute_aux [] e2) lacc s
-   | Thm_THEN e1 e2 \<Rightarrow> s_of_semi__thm_attribute_aux ((\<open>THEN\<close>, s_of_semi__thm_attribute_aux [] e2) # lacc) e1
+   | Thm_THEN (Thm_thm s) e2 \<Rightarrow> of_semi__thm_attribute_aux_gen (\<open>THEN\<close>, of_semi__thm_attribute_aux [] e2) lacc s
+   | Thm_THEN (Thm_thms s) e2 \<Rightarrow> of_semi__thm_attribute_aux_gen (\<open>THEN\<close>, of_semi__thm_attribute_aux [] e2) lacc s
+   | Thm_THEN e1 e2 \<Rightarrow> of_semi__thm_attribute_aux ((\<open>THEN\<close>, of_semi__thm_attribute_aux [] e2) # lacc) e1
 
-   | Thm_simplified (Thm_thm s) e2 \<Rightarrow> s_of_semi__thm_attribute_aux_gen (\<open>simplified\<close>, s_of_semi__thm_attribute_aux [] e2) lacc s
-   | Thm_simplified (Thm_thms s) e2 \<Rightarrow> s_of_semi__thm_attribute_aux_gen (\<open>simplified\<close>, s_of_semi__thm_attribute_aux [] e2) lacc s
-   | Thm_simplified e1 e2 \<Rightarrow> s_of_semi__thm_attribute_aux ((\<open>simplified\<close>, s_of_semi__thm_attribute_aux [] e2) # lacc) e1
+   | Thm_simplified (Thm_thm s) e2 \<Rightarrow> of_semi__thm_attribute_aux_gen (\<open>simplified\<close>, of_semi__thm_attribute_aux [] e2) lacc s
+   | Thm_simplified (Thm_thms s) e2 \<Rightarrow> of_semi__thm_attribute_aux_gen (\<open>simplified\<close>, of_semi__thm_attribute_aux [] e2) lacc s
+   | Thm_simplified e1 e2 \<Rightarrow> of_semi__thm_attribute_aux ((\<open>simplified\<close>, of_semi__thm_attribute_aux [] e2) # lacc) e1
 
-   | Thm_symmetric (Thm_thm s) \<Rightarrow> s_of_semi__thm_attribute_aux_gen (\<open>symmetric\<close>, \<open>\<close>) lacc s 
-   | Thm_symmetric (Thm_thms s) \<Rightarrow> s_of_semi__thm_attribute_aux_gen (\<open>symmetric\<close>, \<open>\<close>) lacc s
-   | Thm_symmetric e1 \<Rightarrow> s_of_semi__thm_attribute_aux ((\<open>symmetric\<close>, \<open>\<close>) # lacc) e1
+   | Thm_symmetric (Thm_thm s) \<Rightarrow> of_semi__thm_attribute_aux_gen (\<open>symmetric\<close>, \<open>\<close>) lacc s 
+   | Thm_symmetric (Thm_thms s) \<Rightarrow> of_semi__thm_attribute_aux_gen (\<open>symmetric\<close>, \<open>\<close>) lacc s
+   | Thm_symmetric e1 \<Rightarrow> of_semi__thm_attribute_aux ((\<open>symmetric\<close>, \<open>\<close>) # lacc) e1
 
-   | Thm_where (Thm_thm s) l \<Rightarrow> s_of_semi__thm_attribute_aux_gen (s_of_semi__thm_attribute_aux_gen_where l) lacc s
-   | Thm_where (Thm_thms s) l \<Rightarrow> s_of_semi__thm_attribute_aux_gen (s_of_semi__thm_attribute_aux_gen_where l) lacc s
-   | Thm_where e1 l \<Rightarrow> s_of_semi__thm_attribute_aux (s_of_semi__thm_attribute_aux_gen_where l # lacc) e1
+   | Thm_where (Thm_thm s) l \<Rightarrow> of_semi__thm_attribute_aux_gen (of_semi__thm_attribute_aux_gen_where l) lacc s
+   | Thm_where (Thm_thms s) l \<Rightarrow> of_semi__thm_attribute_aux_gen (of_semi__thm_attribute_aux_gen_where l) lacc s
+   | Thm_where e1 l \<Rightarrow> of_semi__thm_attribute_aux (of_semi__thm_attribute_aux_gen_where l # lacc) e1
 
-   | Thm_of (Thm_thm s) l \<Rightarrow> s_of_semi__thm_attribute_aux_gen (s_of_semi__thm_attribute_aux_gen_of l) lacc s
-   | Thm_of (Thm_thms s) l \<Rightarrow> s_of_semi__thm_attribute_aux_gen (s_of_semi__thm_attribute_aux_gen_of l) lacc s
-   | Thm_of e1 l \<Rightarrow> s_of_semi__thm_attribute_aux (s_of_semi__thm_attribute_aux_gen_of l # lacc) e1
+   | Thm_of (Thm_thm s) l \<Rightarrow> of_semi__thm_attribute_aux_gen (of_semi__thm_attribute_aux_gen_of l) lacc s
+   | Thm_of (Thm_thms s) l \<Rightarrow> of_semi__thm_attribute_aux_gen (of_semi__thm_attribute_aux_gen_of l) lacc s
+   | Thm_of e1 l \<Rightarrow> of_semi__thm_attribute_aux (of_semi__thm_attribute_aux_gen_of l # lacc) e1
 
-   | Thm_OF (Thm_thm s) e2 \<Rightarrow> s_of_semi__thm_attribute_aux_gen (\<open>OF\<close>, s_of_semi__thm_attribute_aux [] e2) lacc s
-   | Thm_OF (Thm_thms s) e2 \<Rightarrow> s_of_semi__thm_attribute_aux_gen (\<open>OF\<close>, s_of_semi__thm_attribute_aux [] e2) lacc s
-   | Thm_OF e1 e2 \<Rightarrow> s_of_semi__thm_attribute_aux ((\<open>OF\<close>, s_of_semi__thm_attribute_aux [] e2) # lacc) e1) e"
+   | Thm_OF (Thm_thm s) e2 \<Rightarrow> of_semi__thm_attribute_aux_gen (\<open>OF\<close>, of_semi__thm_attribute_aux [] e2) lacc s
+   | Thm_OF (Thm_thms s) e2 \<Rightarrow> of_semi__thm_attribute_aux_gen (\<open>OF\<close>, of_semi__thm_attribute_aux [] e2) lacc s
+   | Thm_OF e1 e2 \<Rightarrow> of_semi__thm_attribute_aux ((\<open>OF\<close>, of_semi__thm_attribute_aux [] e2) # lacc) e1) e"
 
-definition "s_of_semi__thm_attribute = s_of_semi__thm_attribute_aux []"
+definition "of_semi__thm_attribute = of_semi__thm_attribute_aux []"
 
-definition "s_of_semi__thm = (\<lambda> Thms_single thy \<Rightarrow> s_of_semi__thm_attribute thy
-                         | Thms_mult thy \<Rightarrow> s_of_semi__thm_attribute thy)"
+definition "of_semi__thm = (\<lambda> Thms_single thy \<Rightarrow> of_semi__thm_attribute thy
+                         | Thms_mult thy \<Rightarrow> of_semi__thm_attribute thy)"
 
-definition "s_of_semi__thm_attribute_l l = String_concat \<open>
-                            \<close> (L.map s_of_semi__thm_attribute l)"
-definition "s_of_semi__thm_attribute_l1 l = String_concat \<open> \<close> (L.map s_of_semi__thm_attribute l)"
+definition "of_semi__thm_attribute_l l = String_concat \<open>
+                            \<close> (L.map of_semi__thm_attribute l)"
+definition "of_semi__thm_attribute_l1 l = String_concat \<open> \<close> (L.map of_semi__thm_attribute l)"
 
-definition "s_of_semi__thm_l l = String_concat \<open> \<close> (L.map s_of_semi__thm l)"
+definition "of_semi__thm_l l = String_concat \<open> \<close> (L.map of_semi__thm l)"
 
-definition "s_of_lemmas _ = (\<lambda> Lemmas_simp_thm simp s l \<Rightarrow>
+definition "of_lemmas _ = (\<lambda> Lemmas_simp_thm simp s l \<Rightarrow>
     sprint3 \<open>lemmas%s%s = %s\<close>\<acute>
       (if String.is_empty s then \<open>\<close> else sprint1 \<open> %s\<close>\<acute> (To_string s))
       (if simp then \<open>[simp,code_unfold]\<close> else \<open>\<close>)
-      (s_of_semi__thm_attribute_l l)
+      (of_semi__thm_attribute_l l)
                                   | Lemmas_simp_thms s l \<Rightarrow>
     sprint2 \<open>lemmas%s [simp,code_unfold] = %s\<close>\<acute>
       (if String.is_empty s then \<open>\<close> else sprint1 \<open> %s\<close>\<acute> (To_string s))
       (String_concat \<open>
                             \<close> (L.map To_string l)))"
 
-definition "(s_of_semi__attrib_genA :: (semi__thm list \<Rightarrow> String.literal)
+definition "(of_semi__attrib_genA :: (semi__thm list \<Rightarrow> String.literal)
    \<Rightarrow> String.literal \<Rightarrow> semi__thm list \<Rightarrow> String.literal) f attr l = (* error reflection: to be merged *)
  (if l = [] then
     \<open>\<close>
   else
     sprint2 \<open> %s: %s\<close>\<acute> attr (f l))"
 
-definition "(s_of_semi__attrib_genB :: (string list \<Rightarrow> String.literal)
+definition "(of_semi__attrib_genB :: (string list \<Rightarrow> String.literal)
    \<Rightarrow> String.literal \<Rightarrow> string list \<Rightarrow> String.literal) f attr l = (* error reflection: to be merged *)
  (if l = [] then
     \<open>\<close>
   else
     sprint2 \<open> %s: %s\<close>\<acute> attr (f l))"
 
-definition "s_of_semi__attrib = s_of_semi__attrib_genA s_of_semi__thm_l"
-definition "s_of_semi__attrib1 = s_of_semi__attrib_genB (\<lambda>l. String_concat \<open> \<close> (L.map To_string l))"
+definition "of_semi__attrib = of_semi__attrib_genA of_semi__thm_l"
+definition "of_semi__attrib1 = of_semi__attrib_genB (\<lambda>l. String_concat \<open> \<close> (L.map To_string l))"
 
-fun s_of_semi__method where "s_of_semi__method expr = (\<lambda>
+fun of_semi__method where "of_semi__method expr = (\<lambda>
     Method_rule o_s \<Rightarrow> sprint1 \<open>rule%s\<close>\<acute> (case o_s of None \<Rightarrow> \<open>\<close>
-                                                    | Some s \<Rightarrow> sprint1 \<open> %s\<close>\<acute> (s_of_semi__thm_attribute s))
-  | Method_drule s \<Rightarrow> sprint1 \<open>drule %s\<close>\<acute> (s_of_semi__thm_attribute s)
-  | Method_erule s \<Rightarrow> sprint1 \<open>erule %s\<close>\<acute> (s_of_semi__thm_attribute s)
-  | Method_intro l \<Rightarrow> sprint1 \<open>intro %s\<close>\<acute> (s_of_semi__thm_attribute_l1 l)
-  | Method_elim s \<Rightarrow> sprint1 \<open>elim %s\<close>\<acute> (s_of_semi__thm_attribute s)
+                                                    | Some s \<Rightarrow> sprint1 \<open> %s\<close>\<acute> (of_semi__thm_attribute s))
+  | Method_drule s \<Rightarrow> sprint1 \<open>drule %s\<close>\<acute> (of_semi__thm_attribute s)
+  | Method_erule s \<Rightarrow> sprint1 \<open>erule %s\<close>\<acute> (of_semi__thm_attribute s)
+  | Method_intro l \<Rightarrow> sprint1 \<open>intro %s\<close>\<acute> (of_semi__thm_attribute_l1 l)
+  | Method_elim s \<Rightarrow> sprint1 \<open>elim %s\<close>\<acute> (of_semi__thm_attribute s)
   | Method_subst asm l s =>
       let s_asm = if asm then \<open>(asm) \<close> else \<open>\<close> in
       if L.map String.to_list l = [''0''] then
-        sprint2 \<open>subst %s%s\<close>\<acute> s_asm (s_of_semi__thm_attribute s)
+        sprint2 \<open>subst %s%s\<close>\<acute> s_asm (of_semi__thm_attribute s)
       else
-        sprint3 \<open>subst %s(%s) %s\<close>\<acute> s_asm (String_concat \<open> \<close> (L.map To_string l)) (s_of_semi__thm_attribute s)
-  | Method_insert l => sprint1 \<open>insert %s\<close>\<acute> (s_of_semi__thm_l l)
-  | Method_plus t \<Rightarrow> sprint1 \<open>(%s)+\<close>\<acute> (String_concat \<open>, \<close> (List.map s_of_semi__method t))
-  | Method_option t \<Rightarrow> sprint1 \<open>(%s)?\<close>\<acute> (String_concat \<open>, \<close> (List.map s_of_semi__method t))
-  | Method_or t \<Rightarrow> sprint1 \<open>(%s)\<close>\<acute> (String_concat \<open> | \<close> (List.map s_of_semi__method t))
-  | Method_one (Method_simp_only l) \<Rightarrow> sprint1 \<open>simp only: %s\<close>\<acute> (s_of_semi__thm_l l)
+        sprint3 \<open>subst %s(%s) %s\<close>\<acute> s_asm (String_concat \<open> \<close> (L.map To_string l)) (of_semi__thm_attribute s)
+  | Method_insert l => sprint1 \<open>insert %s\<close>\<acute> (of_semi__thm_l l)
+  | Method_plus t \<Rightarrow> sprint1 \<open>(%s)+\<close>\<acute> (String_concat \<open>, \<close> (List.map of_semi__method t))
+  | Method_option t \<Rightarrow> sprint1 \<open>(%s)?\<close>\<acute> (String_concat \<open>, \<close> (List.map of_semi__method t))
+  | Method_or t \<Rightarrow> sprint1 \<open>(%s)\<close>\<acute> (String_concat \<open> | \<close> (List.map of_semi__method t))
+  | Method_one (Method_simp_only l) \<Rightarrow> sprint1 \<open>simp only: %s\<close>\<acute> (of_semi__thm_l l)
   | Method_one (Method_simp_add_del_split l1 l2 []) \<Rightarrow> sprint2 \<open>simp%s%s\<close>\<acute>
-      (s_of_semi__attrib \<open>add\<close> l1)
-      (s_of_semi__attrib \<open>del\<close> l2)
+      (of_semi__attrib \<open>add\<close> l1)
+      (of_semi__attrib \<open>del\<close> l2)
   | Method_one (Method_simp_add_del_split l1 l2 l3) \<Rightarrow> sprint3 \<open>simp%s%s%s\<close>\<acute>
-      (s_of_semi__attrib \<open>add\<close> l1)
-      (s_of_semi__attrib \<open>del\<close> l2)
-      (s_of_semi__attrib \<open>split\<close> l3)
-  | Method_all (Method_simp_only l) \<Rightarrow> sprint1 \<open>simp_all only: %s\<close>\<acute> (s_of_semi__thm_l l)
+      (of_semi__attrib \<open>add\<close> l1)
+      (of_semi__attrib \<open>del\<close> l2)
+      (of_semi__attrib \<open>split\<close> l3)
+  | Method_all (Method_simp_only l) \<Rightarrow> sprint1 \<open>simp_all only: %s\<close>\<acute> (of_semi__thm_l l)
   | Method_all (Method_simp_add_del_split l1 l2 []) \<Rightarrow> sprint2 \<open>simp_all%s%s\<close>\<acute>
-      (s_of_semi__attrib \<open>add\<close> l1)
-      (s_of_semi__attrib \<open>del\<close> l2)
+      (of_semi__attrib \<open>add\<close> l1)
+      (of_semi__attrib \<open>del\<close> l2)
   | Method_all (Method_simp_add_del_split l1 l2 l3) \<Rightarrow> sprint3 \<open>simp_all%s%s%s\<close>\<acute>
-      (s_of_semi__attrib \<open>add\<close> l1)
-      (s_of_semi__attrib \<open>del\<close> l2)
-      (s_of_semi__attrib \<open>split\<close> l3)
+      (of_semi__attrib \<open>add\<close> l1)
+      (of_semi__attrib \<open>del\<close> l2)
+      (of_semi__attrib \<open>split\<close> l3)
   | Method_auto_simp_add_split l_simp l_split \<Rightarrow> sprint2 \<open>auto%s%s\<close>\<acute>
-      (s_of_semi__attrib \<open>simp\<close> l_simp)
-      (s_of_semi__attrib1 \<open>split\<close> l_split)
+      (of_semi__attrib \<open>simp\<close> l_simp)
+      (of_semi__attrib1 \<open>split\<close> l_split)
   | Method_rename_tac l \<Rightarrow> sprint1 \<open>rename_tac %s\<close>\<acute> (String_concat \<open> \<close> (L.map To_string l))
-  | Method_case_tac e \<Rightarrow> sprint1 \<open>case_tac \"%s\"\<close>\<acute> (s_of_semi__term e)
+  | Method_case_tac e \<Rightarrow> sprint1 \<open>case_tac \"%s\"\<close>\<acute> (of_semi__term e)
   | Method_blast None \<Rightarrow> sprint0 \<open>blast\<close>\<acute>
   | Method_blast (Some n) \<Rightarrow> sprint1 \<open>blast %d\<close>\<acute> (To_nat n)
   | Method_clarify \<Rightarrow> sprint0 \<open>clarify\<close>\<acute>
   | Method_metis l_opt l \<Rightarrow> sprint2 \<open>metis %s%s\<close>\<acute> (if l_opt = [] then \<open>\<close>
                                                    else
-                                                     sprint1 \<open>(%s) \<close>\<acute> (String_concat \<open>, \<close> (L.map To_string l_opt))) (s_of_semi__thm_attribute_l1 l)) expr"
+                                                     sprint1 \<open>(%s) \<close>\<acute> (String_concat \<open>, \<close> (L.map To_string l_opt))) (of_semi__thm_attribute_l1 l)) expr"
 
-definition "s_of_semi__command_final = (\<lambda> Command_done \<Rightarrow> \<open>done\<close>
-                                   | Command_by l_apply \<Rightarrow> sprint1 \<open>by(%s)\<close>\<acute> (String_concat \<open>, \<close> (L.map s_of_semi__method l_apply))
+definition "of_semi__command_final = (\<lambda> Command_done \<Rightarrow> \<open>done\<close>
+                                   | Command_by l_apply \<Rightarrow> sprint1 \<open>by(%s)\<close>\<acute> (String_concat \<open>, \<close> (L.map of_semi__method l_apply))
                                    | Command_sorry \<Rightarrow> \<open>sorry\<close>)"
 
-definition "s_of_semi__command_state = (
+definition "of_semi__command_state = (
   \<lambda> Command_apply_end [] \<Rightarrow> \<open>\<close>
   | Command_apply_end l_apply \<Rightarrow> sprint1 \<open>  apply_end(%s)
-\<close>\<acute> (String_concat \<open>, \<close> (L.map s_of_semi__method l_apply)))"
+\<close>\<acute> (String_concat \<open>, \<close> (L.map of_semi__method l_apply)))"
 
-definition' \<open>s_of_semi__command_proof = (
+definition' \<open>of_semi__command_proof = (
   let thesis = \<open>?thesis\<close>
     ; scope_thesis_gen = sprint2 \<open>  proof - %s show %s
 \<close>\<acute>
     ; scope_thesis = \<lambda>s. scope_thesis_gen s thesis in
   \<lambda> Command_apply [] \<Rightarrow> \<open>\<close>
   | Command_apply l_apply \<Rightarrow> sprint1 \<open>  apply(%s)
-\<close>\<acute> (String_concat \<open>, \<close> (L.map s_of_semi__method l_apply))
+\<close>\<acute> (String_concat \<open>, \<close> (L.map of_semi__method l_apply))
   | Command_using l \<Rightarrow> sprint1 \<open>  using %s
-\<close>\<acute> (s_of_semi__thm_l l)
+\<close>\<acute> (of_semi__thm_l l)
   | Command_unfolding l \<Rightarrow> sprint1 \<open>  unfolding %s
-\<close>\<acute> (s_of_semi__thm_l l)
-  | Command_let e_name e_body \<Rightarrow> scope_thesis (sprint2 \<open>let %s = "%s"\<close>\<acute> (s_of_semi__term e_name) (s_of_semi__term e_body))
-  | Command_have n b e e_last \<Rightarrow> scope_thesis (sprint4 \<open>have %s%s: "%s" %s\<close>\<acute> (To_string n) (if b then \<open>[simp]\<close> else \<open>\<close>) (s_of_semi__term e) (s_of_semi__command_final e_last))
+\<close>\<acute> (of_semi__thm_l l)
+  | Command_let e_name e_body \<Rightarrow> scope_thesis (sprint2 \<open>let %s = "%s"\<close>\<acute> (of_semi__term e_name) (of_semi__term e_body))
+  | Command_have n b e e_last \<Rightarrow> scope_thesis (sprint4 \<open>have %s%s: "%s" %s\<close>\<acute> (To_string n) (if b then \<open>[simp]\<close> else \<open>\<close>) (of_semi__term e) (of_semi__command_final e_last))
   | Command_fix_let l l_let o_show _ \<Rightarrow>
       scope_thesis_gen
         (sprint2 \<open>fix %s%s\<close>\<acute> (String_concat \<open> \<close> (L.map To_string l))
@@ -282,20 +282,20 @@ definition' \<open>s_of_semi__command_proof = (
 \<close>                                        )
                                        (L.map
                                          (\<lambda>(e_name, e_body).
-                                           sprint2 \<open>          let %s = "%s"\<close>\<acute> (s_of_semi__term e_name) (s_of_semi__term e_body))
+                                           sprint2 \<open>          let %s = "%s"\<close>\<acute> (of_semi__term e_name) (of_semi__term e_body))
                                          l_let)))
         (case o_show of None \<Rightarrow> thesis
-                      | Some l_show \<Rightarrow> sprint1 \<open>"%s"\<close>\<acute> (String_concat \<open> \<Longrightarrow> \<close> (L.map s_of_semi__term l_show))))\<close>
+                      | Some l_show \<Rightarrow> sprint1 \<open>"%s"\<close>\<acute> (String_concat \<open> \<Longrightarrow> \<close> (L.map of_semi__term l_show))))\<close>
 
-definition "s_of_lemma _ =
+definition "of_lemma _ =
  (\<lambda> Lemma n l_spec l_apply tactic_last \<Rightarrow>
     sprint4 \<open>lemma %s : \"%s\"
 %s%s\<close>\<acute>
       (To_string n)
-      (String_concat \<open> \<Longrightarrow> \<close> (L.map s_of_semi__term l_spec))
+      (String_concat \<open> \<Longrightarrow> \<close> (L.map of_semi__term l_spec))
       (String_concat \<open>\<close> (L.map (\<lambda> [] \<Rightarrow> \<open>\<close> | l_apply \<Rightarrow> sprint1 \<open>  apply(%s)
-\<close>\<acute> (String_concat \<open>, \<close> (L.map s_of_semi__method l_apply))) l_apply))
-      (s_of_semi__command_final tactic_last)
+\<close>\<acute> (String_concat \<open>, \<close> (L.map of_semi__method l_apply))) l_apply))
+      (of_semi__command_final tactic_last)
   | Lemma_assumes n l_spec concl l_apply tactic_last \<Rightarrow>
     sprint5 \<open>lemma %s : %s
 %s%s %s\<close>\<acute>
@@ -305,12 +305,12 @@ definition "s_of_lemma _ =
 assumes %s\"%s\"\<close>\<acute>
             (let (n, b) = if b then (sprint1 \<open>%s[simp]\<close>\<acute> (To_string n), False) else (To_string n, String.is_empty n) in
              if b then \<open>\<close> else sprint1 \<open>%s: \<close>\<acute> n)
-            (s_of_semi__term e)) l_spec
+            (of_semi__term e)) l_spec
        @@@@
        [sprint1 \<open>
-shows \"%s\"\<close>\<acute> (s_of_semi__term concl)]))
-      (String_concat \<open>\<close> (L.map s_of_semi__command_proof l_apply))
-      (s_of_semi__command_final tactic_last)
+shows \"%s\"\<close>\<acute> (of_semi__term concl)]))
+      (String_concat \<open>\<close> (L.map of_semi__command_proof l_apply))
+      (of_semi__command_final tactic_last)
       (String_concat \<open> \<close>
         (L.map
           (\<lambda>l_apply_e.
@@ -319,56 +319,56 @@ shows \"%s\"\<close>\<acute> (s_of_semi__term concl)]))
                  \<open>\<close>
                else
                  sprint1 \<open>
-%s \<close>\<acute> (String_concat \<open>\<close> (L.map s_of_semi__command_state l_apply_e))))
+%s \<close>\<acute> (String_concat \<open>\<close> (L.map of_semi__command_state l_apply_e))))
           (List.map_filter
             (\<lambda> Command_let _ _ \<Rightarrow> Some [] | Command_have _ _ _ _ \<Rightarrow> Some [] | Command_fix_let _ _ _ l \<Rightarrow> Some l | _ \<Rightarrow> None)
             (rev l_apply)))))"
 
 
-definition "s_of_axiomatization _ = (\<lambda> Axiomatization n e \<Rightarrow> sprint2 \<open>axiomatization where %s:
-\"%s\"\<close>\<acute> (To_string n) (s_of_semi__term e))"
+definition "of_axiomatization _ = (\<lambda> Axiomatization n e \<Rightarrow> sprint2 \<open>axiomatization where %s:
+\"%s\"\<close>\<acute> (To_string n) (of_semi__term e))"
 
-definition "s_of_section _ = (\<lambda> Section n section_title \<Rightarrow>
+definition "of_section _ = (\<lambda> Section n section_title \<Rightarrow>
     sprint2 \<open>%s{* %s *}\<close>\<acute>
       (sprint1 \<open>%ssection\<close>\<acute> (if n = 0 then \<open>\<close>
                              else if n = 1 then \<open>sub\<close>
                              else \<open>subsub\<close>))
       (To_string section_title))"
 
-definition "s_of_text _ = (\<lambda> Text s \<Rightarrow> sprint1 \<open>text{* %s *}\<close>\<acute> (To_string s))"
+definition "of_text _ = (\<lambda> Text s \<Rightarrow> sprint1 \<open>text{* %s *}\<close>\<acute> (To_string s))"
 
-definition "s_of_ML _ = (\<lambda> SML e \<Rightarrow> sprint1 \<open>ML{* %s *}\<close>\<acute> (s_of_sexpr e))"
+definition "of_ML _ = (\<lambda> SML e \<Rightarrow> sprint1 \<open>ML{* %s *}\<close>\<acute> (of_sexpr e))"
 
-definition "s_of_thm _ = (\<lambda> Thm thm \<Rightarrow> sprint1 \<open>thm %s\<close>\<acute> (s_of_semi__thm_attribute_l1 thm))"
+definition "of_thm _ = (\<lambda> Thm thm \<Rightarrow> sprint1 \<open>thm %s\<close>\<acute> (of_semi__thm_attribute_l1 thm))"
 
-definition' \<open>s_of_interpretation _ = (\<lambda> Interpretation n loc_n loc_param tac \<Rightarrow>
+definition' \<open>of_interpretation _ = (\<lambda> Interpretation n loc_n loc_param tac \<Rightarrow>
   sprint4 \<open>interpretation %s: %s%s
 %s\<close>\<acute> (To_string n)
      (To_string loc_n)
-     (String_concat \<open>\<close> (L.map (\<lambda>s. sprint1 \<open> "%s"\<close>\<acute> (s_of_semi__term s)) loc_param))
-     (s_of_semi__command_final tac))\<close>
+     (String_concat \<open>\<close> (L.map (\<lambda>s. sprint1 \<open> "%s"\<close>\<acute> (of_semi__term s)) loc_param))
+     (of_semi__command_final tac))\<close>
 
-definition "s_of_semi__t ocl =
-            (\<lambda> Theory_datatype dataty \<Rightarrow> s_of_datatype ocl dataty
-             | Theory_type_synonym ty_synonym \<Rightarrow> s_of_type_synonym ocl ty_synonym
-             | Theory_type_notation ty_notation \<Rightarrow> s_of_type_notation ocl ty_notation
-             | Theory_instantiation instantiation_class \<Rightarrow> s_of_instantiation ocl instantiation_class
-             | Theory_defs defs_overloaded \<Rightarrow> s_of_defs ocl defs_overloaded
-             | Theory_consts consts_class \<Rightarrow> s_of_consts ocl consts_class
-             | Theory_definition definition_hol \<Rightarrow> s_of_definition ocl definition_hol
-             | Theory_lemmas lemmas_simp \<Rightarrow> s_of_lemmas ocl lemmas_simp
-             | Theory_lemma lemma_by \<Rightarrow> s_of_lemma ocl lemma_by
-             | Theory_axiomatization axiom \<Rightarrow> s_of_axiomatization ocl axiom
-             | Theory_section section_title \<Rightarrow> s_of_section ocl section_title
-             | Theory_text text \<Rightarrow> s_of_text ocl text
-             | Theory_ML ml \<Rightarrow> s_of_ML ocl ml
-             | Theory_thm thm \<Rightarrow> s_of_thm ocl thm
-             | Theory_interpretation thm \<Rightarrow> s_of_interpretation ocl thm)"
+definition "of_semi__t ocl =
+            (\<lambda> Theory_datatype dataty \<Rightarrow> of_datatype ocl dataty
+             | Theory_type_synonym ty_synonym \<Rightarrow> of_type_synonym ocl ty_synonym
+             | Theory_type_notation ty_notation \<Rightarrow> of_type_notation ocl ty_notation
+             | Theory_instantiation instantiation_class \<Rightarrow> of_instantiation ocl instantiation_class
+             | Theory_defs defs_overloaded \<Rightarrow> of_defs ocl defs_overloaded
+             | Theory_consts consts_class \<Rightarrow> of_consts ocl consts_class
+             | Theory_definition definition_hol \<Rightarrow> of_definition ocl definition_hol
+             | Theory_lemmas lemmas_simp \<Rightarrow> of_lemmas ocl lemmas_simp
+             | Theory_lemma lemma_by \<Rightarrow> of_lemma ocl lemma_by
+             | Theory_axiomatization axiom \<Rightarrow> of_axiomatization ocl axiom
+             | Theory_section section_title \<Rightarrow> of_section ocl section_title
+             | Theory_text text \<Rightarrow> of_text ocl text
+             | Theory_ML ml \<Rightarrow> of_ML ocl ml
+             | Theory_thm thm \<Rightarrow> of_thm ocl thm
+             | Theory_interpretation thm \<Rightarrow> of_interpretation ocl thm)"
 
 definition "String_concat_map s f l = String_concat s (L.map f l)"
 
-definition' \<open>s_of_semi__theory ocl =
- (\<lambda> H_thy_simple t \<Rightarrow> s_of_semi__t ocl t
+definition' \<open>of_semi__theory ocl =
+ (\<lambda> H_thy_simple t \<Rightarrow> of_semi__t ocl t
   | H_thy_locale data l \<Rightarrow> 
       sprint3 \<open>locale %s =
 %s
@@ -380,59 +380,59 @@ end\<close>\<acute>   (To_string (HolThyLocale_name data))
 \<close>
            (\<lambda> (l_fix, o_assum).
                 sprint2 \<open>%s%s\<close>\<acute> (String_concat_map \<open>
-\<close> (\<lambda>(e, ty). sprint2 \<open>fixes "%s" :: "%s"\<close>\<acute> (s_of_semi__term e) (s_of_semi__typ ty)) l_fix)
+\<close> (\<lambda>(e, ty). sprint2 \<open>fixes "%s" :: "%s"\<close>\<acute> (of_semi__term e) (of_semi__typ ty)) l_fix)
                                 (case o_assum of None \<Rightarrow> \<open>\<close>
                                                | Some (name, e) \<Rightarrow> sprint2 \<open>
-assumes %s: "%s"\<close>\<acute> (To_string name) (s_of_semi__term e)))
+assumes %s: "%s"\<close>\<acute> (To_string name) (of_semi__term e)))
            (HolThyLocale_header data))
         (String_concat_map \<open>
 
 \<close> (String_concat_map \<open>
 
-\<close> (s_of_semi__t ocl)) l))\<close>
+\<close> (of_semi__t ocl)) l))\<close>
 
 end
 
 lemmas [code] =
   (* def *)
-  Print.s_of_datatype_def
-  Print.s_of_type_synonym_def
-  Print.s_of_type_notation_def
-  Print.s_of_instantiation_def
-  Print.s_of_defs_def
-  Print.s_of_consts_def
-  Print.s_of_definition_def
-  Print.s_of_semi__thm_attribute_aux_gen_def
-  Print.s_of_semi__thm_attribute_aux_gen_where_def
-  Print.s_of_semi__thm_attribute_aux_gen_of_def
-  Print.s_of_semi__thm_attribute_def
-  Print.s_of_semi__thm_def
-  Print.s_of_semi__thm_attribute_l_def
-  Print.s_of_semi__thm_attribute_l1_def
-  Print.s_of_semi__thm_l_def
-  Print.s_of_lemmas_def
-  Print.s_of_semi__attrib_genA_def
-  Print.s_of_semi__attrib_genB_def
-  Print.s_of_semi__attrib_def
-  Print.s_of_semi__attrib1_def
-  Print.s_of_semi__command_final_def
-  Print.s_of_semi__command_state_def
-  Print.s_of_semi__command_proof_def
-  Print.s_of_lemma_def
-  Print.s_of_axiomatization_def
-  Print.s_of_section_def
-  Print.s_of_text_def
-  Print.s_of_ML_def
-  Print.s_of_thm_def
-  Print.s_of_interpretation_def
-  Print.s_of_semi__t_def
+  Print.of_datatype_def
+  Print.of_type_synonym_def
+  Print.of_type_notation_def
+  Print.of_instantiation_def
+  Print.of_defs_def
+  Print.of_consts_def
+  Print.of_definition_def
+  Print.of_semi__thm_attribute_aux_gen_def
+  Print.of_semi__thm_attribute_aux_gen_where_def
+  Print.of_semi__thm_attribute_aux_gen_of_def
+  Print.of_semi__thm_attribute_def
+  Print.of_semi__thm_def
+  Print.of_semi__thm_attribute_l_def
+  Print.of_semi__thm_attribute_l1_def
+  Print.of_semi__thm_l_def
+  Print.of_lemmas_def
+  Print.of_semi__attrib_genA_def
+  Print.of_semi__attrib_genB_def
+  Print.of_semi__attrib_def
+  Print.of_semi__attrib1_def
+  Print.of_semi__command_final_def
+  Print.of_semi__command_state_def
+  Print.of_semi__command_proof_def
+  Print.of_lemma_def
+  Print.of_axiomatization_def
+  Print.of_section_def
+  Print.of_text_def
+  Print.of_ML_def
+  Print.of_thm_def
+  Print.of_interpretation_def
+  Print.of_semi__t_def
   Print.String_concat_map_def
-  Print.s_of_semi__theory_def
+  Print.of_semi__theory_def
 
   (* fun *)
-  Print.s_of_semi__typ.simps
-  Print.s_of_semi__term.simps
-  Print.s_of_semi__thm_attribute_aux.simps
-  Print.s_of_semi__method.simps
+  Print.of_semi__typ.simps
+  Print.of_semi__term.simps
+  Print.of_semi__thm_attribute_aux.simps
+  Print.of_semi__method.simps
 
 end
