src/compiler_generic/meta_isabelle/Printer_Pure.thy
@@ -46,13 +46,13 @@ begin
 context Print
 begin
 
-fun s_of_pure_term where "s_of_pure_term l e = (\<lambda>
+fun of_pure_term where "of_pure_term l e = (\<lambda>
     Const s _ \<Rightarrow> To_string s
   | Free s _ \<Rightarrow> To_string s
-  | App t1 t2 \<Rightarrow> sprint2 \<open>(%s) (%s)\<close>\<acute> (s_of_pure_term l t1) (s_of_pure_term l t2)
+  | App t1 t2 \<Rightarrow> sprint2 \<open>(%s) (%s)\<close>\<acute> (of_pure_term l t1) (of_pure_term l t2)
   | Abs s _ t \<Rightarrow>
       let s = To_string s in
-      sprint2 \<open>(\<lambda> %s. %s)\<close>\<acute> s (s_of_pure_term (s # l) t)
+      sprint2 \<open>(\<lambda> %s. %s)\<close>\<acute> s (of_pure_term (s # l) t)
   | Bound n \<Rightarrow> sprint1 \<open>%s\<close>\<acute> (l ! nat_of_natural n)) e"
 
 end
@@ -60,6 +60,6 @@ end
 lemmas [code] =
   (* def *)
   (* fun *)
-  Print.s_of_pure_term.simps
+  Print.of_pure_term.simps
 
 end
