src/compiler_generic/toy_example/embedding/meta_toy/Parser_META.thy
@@ -88,64 +88,64 @@ subsubsection{* general *}
 context Parse
 begin
 
-definition "i_of_ocl_flush_all a b = rec_ocl_flush_all
+definition "of_ocl_flush_all a b = rec_ocl_flush_all
   (b \<open>OclFlushAll\<close>)"
 
-definition "i_of_floor a b = rec_floor
+definition "of_floor a b = rec_floor
   (b \<open>Floor1\<close>)
   (b \<open>Floor2\<close>)
   (b \<open>Floor3\<close>)"
 
-definition "i_of_all_meta_embedding a b = rec_all_meta_embedding
-  (ap1 a (b \<open>META_enum\<close>) (i_of_ocl_enum a b))
-  (ap2 a (b \<open>META_class_raw\<close>) (i_of_floor a b) (i_of_ocl_class_raw a b (K i_of_unit)))
-  (ap1 a (b \<open>META_association\<close>) (i_of_ocl_association a b (K i_of_unit)))
-  (ap2 a (b \<open>META_ass_class\<close>) (i_of_floor a b) (i_of_ocl_ass_class a b))
-  (ap2 a (b \<open>META_ctxt\<close>) (i_of_floor a b) (i_of_ocl_ctxt a b (K i_of_unit)))
+definition "of_all_meta_embedding a b = rec_all_meta_embedding
+  (ap1 a (b \<open>META_enum\<close>) (of_ocl_enum a b))
+  (ap2 a (b \<open>META_class_raw\<close>) (of_floor a b) (of_ocl_class_raw a b (K of_unit)))
+  (ap1 a (b \<open>META_association\<close>) (of_ocl_association a b (K of_unit)))
+  (ap2 a (b \<open>META_ass_class\<close>) (of_floor a b) (of_ocl_ass_class a b))
+  (ap2 a (b \<open>META_ctxt\<close>) (of_floor a b) (of_ocl_ctxt a b (K of_unit)))
 
-  (ap1 a (b \<open>META_class_synonym\<close>) (i_of_ocl_class_synonym a b))
-  (ap1 a (b \<open>META_instance\<close>) (i_of_ocl_instance a b))
-  (ap1 a (b \<open>META_def_base_l\<close>) (i_of_ocl_def_base_l a b))
-  (ap2 a (b \<open>META_def_state\<close>) (i_of_floor a b) (i_of_ocl_def_state a b))
-  (ap2 a (b \<open>META_def_pre_post\<close>) (i_of_floor a b) (i_of_ocl_def_pre_post a b))
-  (ap1 a (b \<open>META_flush_all\<close>) (i_of_ocl_flush_all a b))"
+  (ap1 a (b \<open>META_class_synonym\<close>) (of_ocl_class_synonym a b))
+  (ap1 a (b \<open>META_instance\<close>) (of_ocl_instance a b))
+  (ap1 a (b \<open>META_def_base_l\<close>) (of_ocl_def_base_l a b))
+  (ap2 a (b \<open>META_def_state\<close>) (of_floor a b) (of_ocl_def_state a b))
+  (ap2 a (b \<open>META_def_pre_post\<close>) (of_floor a b) (of_ocl_def_pre_post a b))
+  (ap1 a (b \<open>META_flush_all\<close>) (of_ocl_flush_all a b))"
 
-definition "i_of_generation_semantics_ocl a b = rec_generation_semantics_ocl
+definition "of_generation_semantics_ocl a b = rec_generation_semantics_ocl
   (b \<open>Gen_only_design\<close>)
   (b \<open>Gen_only_analysis\<close>)
   (b \<open>Gen_default\<close>)"
 
-definition "i_of_generation_lemma_mode a b = rec_generation_lemma_mode
+definition "of_generation_lemma_mode a b = rec_generation_lemma_mode
   (b \<open>Gen_sorry\<close>)
   (b \<open>Gen_no_dirty\<close>)"
 
-definition "i_of_compiler_env_config a b f = compiler_env_config_rec
+definition "of_compiler_env_config a b f = compiler_env_config_rec
   (ap15 a (b (ext \<open>compiler_env_config_ext\<close>))
-    (i_of_bool b)
-    (i_of_option a b (i_of_pair a b (i_of_string a b) (i_of_pair a b (i_of_list a b (i_of_string a b)) (i_of_string a b))))
-    (i_of_internal_oids a b)
-    (i_of_pair a b (i_of_nat a b) (i_of_nat a b))
-    (i_of_generation_semantics_ocl a b)
-    (i_of_option a b (i_of_ocl_class a b))
-    (i_of_list a b (i_of_all_meta_embedding a b))
-    (i_of_list a b (i_of_pair a b (i_of_string\<^sub>b\<^sub>a\<^sub>s\<^sub>e a b) (i_of_pair a b (i_of_ocl_instance_single a b (K i_of_unit)) (i_of_internal_oids a b))))
-    (i_of_list a b (i_of_pair a b (i_of_string\<^sub>b\<^sub>a\<^sub>s\<^sub>e a b) (i_of_list a b (i_of_pair a b (i_of_internal_oids a b) (i_of_ocl_def_state_core a b (i_of_pair a b (i_of_string a b) (i_of_ocl_instance_single a b  (K i_of_unit))))))))
-    (i_of_bool b)
-    (i_of_bool b)
-    (i_of_pair a b (i_of_list a b (i_of_string\<^sub>b\<^sub>a\<^sub>s\<^sub>e a b)) (i_of_list a b (i_of_string\<^sub>b\<^sub>a\<^sub>s\<^sub>e a b)))
-    (i_of_list a b (i_of_string\<^sub>b\<^sub>a\<^sub>s\<^sub>e a b))
-    (i_of_pair a b (i_of_option a b (i_of_generation_lemma_mode a b)) (i_of_bool b))
+    (of_bool b)
+    (of_option a b (of_pair a b (of_string a b) (of_pair a b (of_list a b (of_string a b)) (of_string a b))))
+    (of_internal_oids a b)
+    (of_pair a b (of_nat a b) (of_nat a b))
+    (of_generation_semantics_ocl a b)
+    (of_option a b (of_ocl_class a b))
+    (of_list a b (of_all_meta_embedding a b))
+    (of_list a b (of_pair a b (of_string\<^sub>b\<^sub>a\<^sub>s\<^sub>e a b) (of_pair a b (of_ocl_instance_single a b (K of_unit)) (of_internal_oids a b))))
+    (of_list a b (of_pair a b (of_string\<^sub>b\<^sub>a\<^sub>s\<^sub>e a b) (of_list a b (of_pair a b (of_internal_oids a b) (of_ocl_def_state_core a b (of_pair a b (of_string a b) (of_ocl_instance_single a b  (K of_unit))))))))
+    (of_bool b)
+    (of_bool b)
+    (of_pair a b (of_list a b (of_string\<^sub>b\<^sub>a\<^sub>s\<^sub>e a b)) (of_list a b (of_string\<^sub>b\<^sub>a\<^sub>s\<^sub>e a b)))
+    (of_list a b (of_string\<^sub>b\<^sub>a\<^sub>s\<^sub>e a b))
+    (of_pair a b (of_option a b (of_generation_lemma_mode a b)) (of_bool b))
     (f a b))"
 
 end
 
 lemmas [code] =
-  Parse.i_of_ocl_flush_all_def
-  Parse.i_of_floor_def
-  Parse.i_of_all_meta_embedding_def
-  Parse.i_of_generation_semantics_ocl_def
-  Parse.i_of_generation_lemma_mode_def
-  Parse.i_of_compiler_env_config_def
+  Parse.of_ocl_flush_all_def
+  Parse.of_floor_def
+  Parse.of_all_meta_embedding_def
+  Parse.of_generation_semantics_ocl_def
+  Parse.of_generation_lemma_mode_def
+  Parse.of_compiler_env_config_def
 
 subsubsection{* Isabelle *}
 
@@ -160,27 +160,27 @@ definition "i_Some = \<open>Some\<close>"
 
 (* *)
 
-definition "i_of_pair a b f1 f2 = (\<lambda>f. \<lambda>(c, d) \<Rightarrow> f c d)
+definition "of_pair a b f1 f2 = (\<lambda>f. \<lambda>(c, d) \<Rightarrow> f c d)
   (ap2 a (b i_Pair) f1 f2)"
 
-definition "i_of_list a b f = (\<lambda>f0. rec_list f0 o co1 K)
+definition "of_list a b f = (\<lambda>f0. rec_list f0 o co1 K)
   (b i_Nil)
   (ar2 a (b i_Cons) f)"
 
-definition "i_of_option a b f = rec_option
+definition "of_option a b f = rec_option
   (b i_None)
   (ap1 a (b i_Some) f)"
 
 (* *)
 
-definition "i_of_unit b = case_unit
+definition "of_unit b = case_unit
   (b \<open>()\<close>)"
 
-definition "i_of_bool b = case_bool
+definition of_bool where "of_bool b = case_bool
   (b \<open>True\<close>)
   (b \<open>False\<close>)"
 
-definition "i_of_nibble b = rec_nibble
+definition "of_nibble b = rec_nibble
   (b \<open>Nibble0\<close>)
   (b \<open>Nibble1\<close>)
   (b \<open>Nibble2\<close>)
@@ -198,37 +198,37 @@ definition "i_of_nibble b = rec_nibble
   (b \<open>NibbleE\<close>)
   (b \<open>NibbleF\<close>)"
 
-definition "i_of_char a b = rec_char
-  (ap2 a (b \<open>Char\<close>) (i_of_nibble b) (i_of_nibble b))"
+definition "of_char a b = rec_char
+  (ap2 a (b \<open>Char\<close>) (of_nibble b) (of_nibble b))"
 
-definition "i_of_string_gen s_flatten s_st0 s_st a b s = 
+definition "of_string_gen s_flatten s_st0 s_st a b s = 
   b (let s = textstr_of_str (\<lambda>c. \<open>(\<close> @@ s_flatten @@ \<open> \<close> @@ c @@ \<open>)\<close>)
                             (\<lambda>Char n1 n2 \<Rightarrow>
-                                 s_st0 (S.flatten [\<open> (\<close>, \<open>Char \<close>, i_of_nibble id n1, \<open> \<close>, i_of_nibble id n2, \<open>)\<close>]))
+                                 s_st0 (S.flatten [\<open> (\<close>, \<open>Char \<close>, of_nibble id n1, \<open> \<close>, of_nibble id n2, \<open>)\<close>]))
                             (\<lambda>c. s_st (S.flatten [\<open> (\<close>, c, \<open>)\<close>]))
                             s in
      S.flatten [ \<open>(\<close>, s, \<open>)\<close> ])"
 
-definition "i_of_string = i_of_string_gen \<open>Init.S.flatten\<close>
+definition "of_string = of_string_gen \<open>Init.S.flatten\<close>
                                           (\<lambda>s. S.flatten [\<open>(Init.ST0\<close>, s, \<open>)\<close>])
                                           (\<lambda>s. S.flatten [\<open>(Init.abr_string.SS_base (Init.string\<^sub>b\<^sub>a\<^sub>s\<^sub>e.ST\<close>, s, \<open>))\<close>])"
-definition "i_of_string\<^sub>b\<^sub>a\<^sub>s\<^sub>e a b s = i_of_string_gen \<open>Init.String\<^sub>b\<^sub>a\<^sub>s\<^sub>e.flatten\<close>
+definition "of_string\<^sub>b\<^sub>a\<^sub>s\<^sub>e a b s = of_string_gen \<open>Init.String\<^sub>b\<^sub>a\<^sub>s\<^sub>e.flatten\<close>
                                                    (\<lambda>s. S.flatten [\<open>(Init.ST0_base\<close>, s, \<open>)\<close>])
                                                    (\<lambda>s. S.flatten [\<open>(Init.string\<^sub>b\<^sub>a\<^sub>s\<^sub>e.ST\<close>, s, \<open>)\<close>])
                                                    a
                                                    b
                                                    (String\<^sub>b\<^sub>a\<^sub>s\<^sub>e.to_String s)"
 
-definition "i_of_nat a b = b o String.of_natural"
+definition of_nat where "of_nat a b = b o String.of_natural"
 
 end
 
 sublocale isabelle_of < Parse "id"
-                              isabelle_of.i_of_string
-                              isabelle_of.i_of_string\<^sub>b\<^sub>a\<^sub>s\<^sub>e
-                              isabelle_of.i_of_nat
-                              isabelle_of.i_of_unit
-                              isabelle_of.i_of_bool
+                              isabelle_of.of_string
+                              isabelle_of.of_string\<^sub>b\<^sub>a\<^sub>s\<^sub>e
+                              isabelle_of.of_nat
+                              isabelle_of.of_unit
+                              isabelle_of.of_bool
                               isabelle_of.i_Pair
                               isabelle_of.i_Nil
                               isabelle_of.i_Cons
@@ -238,10 +238,10 @@ done
 
 context isabelle_of begin
   definition "ocl_embed a b =
-    i_of_compiler_env_config a b (\<lambda> a b.
-      i_of_pair a b
-        (i_of_list a b (i_of_all_meta_embedding a b))
-        (i_of_option a b (i_of_string a b)))"
+    of_compiler_env_config a b (\<lambda> a b.
+      of_pair a b
+        (of_list a b (of_all_meta_embedding a b))
+        (of_option a b (of_string a b)))"
 end
 
 definition "isabelle_of_ocl_embed = isabelle_of.ocl_embed"
@@ -253,17 +253,17 @@ lemmas [code] =
   isabelle_of.i_None_def
   isabelle_of.i_Some_def
 
-  isabelle_of.i_of_pair_def
-  isabelle_of.i_of_list_def
-  isabelle_of.i_of_option_def
-  isabelle_of.i_of_unit_def
-  isabelle_of.i_of_bool_def
-  isabelle_of.i_of_nibble_def
-  isabelle_of.i_of_char_def
-  isabelle_of.i_of_string_gen_def
-  isabelle_of.i_of_string_def
-  isabelle_of.i_of_string\<^sub>b\<^sub>a\<^sub>s\<^sub>e_def
-  isabelle_of.i_of_nat_def
+  isabelle_of.of_pair_def
+  isabelle_of.of_list_def
+  isabelle_of.of_option_def
+  isabelle_of.of_unit_def
+  isabelle_of.of_bool_def
+  isabelle_of.of_nibble_def
+  isabelle_of.of_char_def
+  isabelle_of.of_string_gen_def
+  isabelle_of.of_string_def
+  isabelle_of.of_string\<^sub>b\<^sub>a\<^sub>s\<^sub>e_def
+  isabelle_of.of_nat_def
 
   isabelle_of.ocl_embed_def
 
@@ -284,23 +284,23 @@ definition "i_Some = \<open>SOME\<close>"
 
 (* *)
 
-definition "i_of_pair a b f1 f2 = (\<lambda>f. \<lambda>(c, d) \<Rightarrow> f c d)
+definition "of_pair a b f1 f2 = (\<lambda>f. \<lambda>(c, d) \<Rightarrow> f c d)
   (ap2 a (b i_Pair) f1 f2)"
 
-definition "i_of_list a b f = (\<lambda>f0. rec_list f0 o co1 K)
+definition "of_list a b f = (\<lambda>f0. rec_list f0 o co1 K)
   (b i_Nil)
   (ar2 a (b i_Cons) f)"
 
-definition "i_of_option a b f = rec_option
+definition "of_option a b f = rec_option
   (b i_None)
   (ap1 a (b i_Some) f)"
 
 (* *)
 
-definition "i_of_unit b = case_unit
+definition "of_unit b = case_unit
   (b \<open>()\<close>)"
 
-definition "i_of_bool b = case_bool
+definition of_bool where "of_bool b = case_bool
   (b \<open>true\<close>)
   (b \<open>false\<close>)"
 
@@ -317,26 +317,26 @@ definition' \<open>sml_escape =
                             else if x = Char Nibble7 NibbleF then \<open>\127\<close>
                             else \<degree>x\<degree>)\<close>
 
-definition' \<open>i_of_string a b =
+definition' \<open>of_string a b =
  (\<lambda>x. b (S.flatten [ \<open>(OCL.SS_base (OCL.ST "\<close>
                   , sml_escape x
                   , \<open>"))\<close>]))\<close>
 
-definition' \<open>i_of_string\<^sub>b\<^sub>a\<^sub>s\<^sub>e a b =
+definition' \<open>of_string\<^sub>b\<^sub>a\<^sub>s\<^sub>e a b =
  (\<lambda>x. b (S.flatten [ \<open>(OCL.ST "\<close>
                   , sml_escape (String\<^sub>b\<^sub>a\<^sub>s\<^sub>e.to_String x)
                   , \<open>")\<close>]))\<close>
 
-definition "i_of_nat a b = (\<lambda>x. b (S.flatten [\<open>(Code_Numeral.Nat \<close>, String.of_natural x, \<open>)\<close>]))"
+definition of_nat where "of_nat a b = (\<lambda>x. b (S.flatten [\<open>(Code_Numeral.Nat \<close>, String.of_natural x, \<open>)\<close>]))"
 
 end
 
 sublocale sml_of < Parse "\<lambda>c. case String.to_list c of x # xs \<Rightarrow> S.flatten [String.uppercase \<lless>[x]\<ggreater>, \<lless>xs\<ggreater>]"
-                         sml_of.i_of_string
-                         sml_of.i_of_string\<^sub>b\<^sub>a\<^sub>s\<^sub>e
-                         sml_of.i_of_nat
-                         sml_of.i_of_unit
-                         sml_of.i_of_bool
+                         sml_of.of_string
+                         sml_of.of_string\<^sub>b\<^sub>a\<^sub>s\<^sub>e
+                         sml_of.of_nat
+                         sml_of.of_unit
+                         sml_of.of_bool
                          sml_of.i_Pair
                          sml_of.i_Nil
                          sml_of.i_Cons
@@ -345,7 +345,7 @@ sublocale sml_of < Parse "\<lambda>c. case String.to_list c of x # xs \<Rightarr
 done
 
 context sml_of begin
-  definition "ocl_unit a b = i_of_compiler_env_config a b (\<lambda> _. i_of_unit)"
+  definition "ocl_unit a b = of_compiler_env_config a b (\<lambda> _. of_unit)"
 end
 
 definition "sml_of_ocl_unit = sml_of.ocl_unit"
@@ -357,14 +357,14 @@ lemmas [code] =
   sml_of.i_None_def
   sml_of.i_Some_def
 
-  sml_of.i_of_pair_def
-  sml_of.i_of_list_def
-  sml_of.i_of_option_def
-  sml_of.i_of_unit_def
-  sml_of.i_of_bool_def
-  sml_of.i_of_string_def
-  sml_of.i_of_string\<^sub>b\<^sub>a\<^sub>s\<^sub>e_def
-  sml_of.i_of_nat_def
+  sml_of.of_pair_def
+  sml_of.of_list_def
+  sml_of.of_option_def
+  sml_of.of_unit_def
+  sml_of.of_bool_def
+  sml_of.of_string_def
+  sml_of.of_string\<^sub>b\<^sub>a\<^sub>s\<^sub>e_def
+  sml_of.of_nat_def
 
   sml_of.sml_escape_def
   sml_of.ocl_unit_def
